Dexter2 set_delegate remap (#152)
* Remove implicit serializable argument from FA2, FA1.2 and Dexter2 message definitions

* Fix FA2 callback show instance

* Rename init and receive in Dexter2 lqt and CPMM contracts as a workaround to coq extraction bug

* Move null_address and set_delegate_call  parameters to into module type

* Remap set_delegate_call to Tezos operation in Dexter2 CPMM extraction

* Remap key_hash type

examples/dexter/Dexter.v
@@ -43,7 +43,7 @@ Inductive DexterMsg :=
 Global Instance DexterMsg_serializable : Serializable DexterMsg :=
   Derive Serializable DexterMsg_rect <tokens_to_asset, add_to_tokens_reserve>.
 
-Definition Msg := @FA2ReceiverMsg BaseTypes DexterMsg _.
+Definition Msg := @FA2ReceiverMsg BaseTypes DexterMsg.
 
 
 Record State :=
